ref: no config

DenotationalLean/ADeriv.lean
@@ -4,20 +4,18 @@ import DenotationalLean.State
 
 /-! # 2.2 The evaluation of arithmetic expressions -/
 
-abbrev Config := Aexp × State
-
-inductive a_deriv : Config -> Nat -> Prop
-  | num {n σ} : a_deriv (Aexp.Nat n, σ) n
-  | loc {l σ} : a_deriv (Aexp.Loc l, σ) (State.lookup σ l)
-  | add {a0 n0 a1 n1 σ} : a_deriv (a0,σ) n0 -> a_deriv (a1,σ) n1 -> a_deriv (Aexp.Add a0 a1,σ) (n0+n1)
-  | sub {a0 n0 a1 n1 σ} : a_deriv (a0,σ) n0 -> a_deriv (a1,σ) n1 -> a_deriv (Aexp.Sub a0 a1,σ) (n0-n1)
-  | mul {a0 n0 a1 n1 σ} : a_deriv (a0,σ) n0 -> a_deriv (a1,σ) n1 -> a_deriv (Aexp.Mul a0 a1,σ) (n0*n1)
+inductive a_deriv : Aexp -> State -> Nat -> Prop
+  | num {n σ} : a_deriv (Aexp.Nat n) σ n
+  | loc {l σ} : a_deriv (Aexp.Loc l) σ (State.lookup σ l)
+  | add {a0 n0 a1 n1 σ} : a_deriv a0 σ n0 -> a_deriv a1 σ n1 -> a_deriv (Aexp.Add a0 a1) σ (n0+n1)
+  | sub {a0 n0 a1 n1 σ} : a_deriv a0 σ n0 -> a_deriv a1 σ n1 -> a_deriv (Aexp.Sub a0 a1) σ (n0-n1)
+  | mul {a0 n0 a1 n1 σ} : a_deriv a0 σ n0 -> a_deriv a1 σ n1 -> a_deriv (Aexp.Mul a0 a1) σ (n0*n1)
 
 
 /- example : ⟨(Init + 5) + (7 + 9), σ_0⟩ -> 21 -/
 example : a_deriv
-    ((#"Init" + |5|) + (|7| + |9|),
-    [("Init",0)])
+    ((#"Init" + |5|) + (|7| + |9|))
+    [("Init",0)]
     21 := by
   let σ := [("Init",0)]
   have h0 : State.lookup σ "Init" = 0 := by rfl
@@ -32,12 +30,12 @@ example : a_deriv
   assumption
 
 def a_equiv (a0 a1 : Aexp) : Prop :=
-  ∀ (n : Nat) (σ : State) , (a_deriv (a0,σ) n) <-> (a_deriv (a1,σ) n)
+  ∀ (n : Nat) (σ : State) , (a_deriv a0 σ n) <-> (a_deriv a1 σ n)
 
 /- Proposition 3.3 -/
 
 theorem a_unique (a : Aexp) (σ : State) :
-    ∀ (n0 n1 : Nat) , a_deriv (a,σ) n0 ∧ a_deriv (a,σ) n1 -> n0 = n1 := by
+    ∀ (n0 n1 : Nat) , a_deriv a σ n0 ∧ a_deriv a σ n1 -> n0 = n1 := by
   induction a <;>
   intro n0 n1 <;> intro ⟨h0,h1⟩ <;>
   cases h0 <;> cases h1 <;> grind
@@ -52,7 +50,7 @@ def a_eval (a : Aexp) (σ : State) : Nat :=
   | .Sub a0 a1 => a_eval a0 σ - a_eval a1 σ
   | .Mul a0 a1 => a_eval a0 σ * a_eval a1 σ
 
-theorem a_eval_deriv (a : Aexp) (σ : State) : a_deriv (a,σ) (a_eval a σ) :=
+theorem a_eval_deriv (a : Aexp) (σ : State) : a_deriv a σ (a_eval a σ) :=
   match a with
   | .Nat _ => a_deriv.num
   | .Loc _ => a_deriv.loc
